Refactor a bit, work on side conditions for let expansion

pcuic/theories/PCUICEtaExpand.v
@@ -1,7 +1,42 @@
-From Coq Require Import ssreflect.
+From Coq Require Import ssreflect ssrbool.
 From Equations Require Import Equations.
 From MetaCoq.Utils Require Import utils.
-From MetaCoq.PCUIC Require Import PCUICAst PCUICAstUtils PCUICTyping PCUICProgram PCUICCSubst.
+From MetaCoq.Common Require Import config.
+From MetaCoq.PCUIC Require Import PCUICAst PCUICAstUtils PCUICTyping
+  PCUICReduction PCUICProgram PCUICLiftSubst PCUICCSubst PCUICUnivSubst.
+
+(* todo move *)
+Lemma All_fold_tip {A : Type} (P : list A -> A -> Type) {x} : All_fold P [x] -> P [] x.
+Proof.
+  intros a; now depelim a.
+Qed.
+
+Lemma All_tip {A} {P : A -> Type} {a : A} : P a <~> All P [a].
+Proof. split; intros. repeat constructor; auto. now depelim X. Qed.
+
+Lemma nApp_mkApps t f args :
+  t = mkApps f args -> ~~ isApp t -> t = f /\ args = [].
+Proof.
+  intros -> napp.
+  destruct args using rev_case; cbn in *; solve_discr; try discriminate => //. split => //.
+  now rewrite mkApps_app /= in napp.
+Qed.
+
+Ltac solve_discr :=
+  try progress (prepare_discr; finish_discr; cbn[mkApps] in * );
+  try match goal with
+    H : mkApps _ _ = mkApps ?f ?l |- _ =>
+    eapply mkApps_eq_inj in H as [? ?]; [|easy|easy]; subst; try intuition congruence; try noconf H
+  | H : ?t = mkApps ?f ?l |- _ =>
+    (change t with (mkApps t []) in H ;
+    eapply mkApps_eq_inj in H as [? ?]; [|easy|easy]; subst; try intuition congruence; try noconf H) ||
+    (eapply nApp_mkApps in H as [? ?]; [|easy]; subst)
+  | H : mkApps ?f ?l = ?t |- _ =>
+    change t with (mkApps t []) in H ;
+    eapply mkApps_eq_inj in H as [? ?]; [|easy|easy]; subst; try intuition congruence; try noconf H
+  end.
+
+(* end move *)
 
 Definition isConstruct t :=
    match t with tConstruct _ _ _ => true | _ => false end.
@@ -188,10 +223,6 @@ Definition expanded_global_env (g : global_env) :=
 Definition expanded_pcuic_program (p : pcuic_program) :=
   expanded_global_env p.1 /\ expanded p.1 [] p.2.
 
-
-Lemma All_tip {A} {P : A -> Type} {a : A} : P a <~> All P [a].
-Proof. split; intros. repeat constructor; auto. now depelim X. Qed.
-
 Lemma expanded_mkApps_expanded {Σ Γ f args} :
   expanded Σ Γ f -> All (expanded Σ Γ) args ->
   expanded Σ Γ (mkApps f args).
@@ -200,15 +231,11 @@ Proof.
   destruct (isConstruct f || isFix f || isRel f) eqn:eqc.
   destruct f => //.
   - depelim H; solve_discr. eapply expanded_tRel; tea. cbn in Hle. lia. solve_all.
-    destruct args0 using rev_case; cbn in *; subst. cbn in H. congruence.
-    rewrite mkApps_app in H2; noconf H2.
+    now rewrite eqc in H.
   - depelim H; solve_discr.
-    destruct args0 using rev_case; cbn in *; subst. cbn in H. congruence.
-    rewrite mkApps_app in H2; noconf H2.
+    now rewrite eqc in H.
     eapply expanded_tConstruct_app; tea. cbn in H0. lia. solve_all.
-  - depelim H; solve_discr.
-    destruct args0 using rev_case; cbn in *; subst. cbn in H. congruence.
-    rewrite mkApps_app in H2; noconf H2.
+  - depelim H; solve_discr. now rewrite eqc in H.
   - eapply expanded_mkApps. now rewrite eqc. auto. solve_all.
 Qed.
 
@@ -341,19 +368,6 @@ Proof.
     solve_all.
 Qed.
 
-Lemma csubst_mkApps a k f l :
-  csubst a k (mkApps f l) = mkApps (csubst a k f) (map (csubst a k) l).
-Proof.
-  induction l in f |- *; cbn; [auto|].
-  rewrite IHl.
-  now cbn.
-Qed.
-
-Lemma All_fold_tip {A : Type} (P : list A -> A -> Type) {x} : All_fold P [x] -> P [] x.
-Proof.
-  intros a; now depelim a.
-Qed.
-
 Lemma expanded_let_expansion Σ (Δ : context) Γ t :
   expanded_context Σ Γ Δ ->
   expanded Σ (repeat 0 #|Δ| ++ Γ) t ->
@@ -394,8 +408,6 @@ Proof.
       exact exp. lia.
 Qed.
 
-Require Import PCUICUnivSubst.
-
 Lemma subst_instance_isConstruct t u : isConstruct t@[u] = isConstruct t.
 Proof. destruct t => //. Qed.
 Lemma subst_instance_isRel t u : isRel t@[u] = isRel t.
@@ -432,5 +444,927 @@ Proof.
      now eapply nth_error_Some_length in H. assumption.
     solve_all. }
   all:intros; try solve [econstructor; eauto 1; solve_all; try now rewrite app_assoc].
+Qed.
+
+
+Lemma expanded_tApp (Σ : global_env) (Γ : list nat) (f : term) a :
+  expanded Σ Γ f -> expanded Σ Γ a ->
+  expanded Σ Γ (tApp f a).
+Proof.
+  induction 1 using expanded_ind; intros expa.
+  all:rewrite -?[tApp _ a](mkApps_app _ _ [a]).
+  all:try (eapply (expanded_mkApps _ _ _ [a]) => //; econstructor; eauto).
+
+  - econstructor; tea. rewrite app_length. lia. eapply app_Forall;eauto.
+  - econstructor; tea. eapply app_Forall; eauto.
+  - eapply expanded_tFix; tea. eapply app_Forall; eauto. eauto. rewrite app_length; cbn; eauto. lia.
+  - eapply expanded_tConstruct_app; tea. rewrite app_length ; lia. eapply app_Forall; eauto.
+Qed.
+
+Lemma expanded_tApp_inv Σ Γ f a :
+  ~ isConstruct (head f) || isFix (head f) || isRel (head f) ->
+  expanded Σ Γ (tApp f a) ->
+  expanded Σ Γ f /\ expanded Σ Γ a.
+Proof.
+  intros hf exp; depind exp.
+  - destruct args using rev_case; solve_discr; try discriminate.
+    rewrite mkApps_app in H3; noconf H3.
+    eapply Forall_app in H1 as [? ha]. depelim ha.
+    destruct args using rev_case; cbn in hf => //.
+    now rewrite !head_mkApps /= in hf.
+  - destruct args using rev_case; solve_discr. subst f6.
+    eapply IHexp => //.
+    rewrite mkApps_app in H2; noconf H2.
+    eapply Forall_app in H0 as [? H0]. depelim H0. split => //.
+    rewrite !head_mkApps in hf.
+    eapply expanded_mkApps => //.
+  - destruct args using rev_case; solve_discr. discriminate.
+    rewrite mkApps_app in H6; noconf H6.
+    eapply Forall_app in H1 as [? h]. depelim h. split => //.
+    now rewrite !head_mkApps /= in hf.
+  - destruct args using rev_case; solve_discr. discriminate.
+    rewrite mkApps_app in H3; noconf H3.
+    now rewrite !head_mkApps /= in hf.
+Qed.
+
+Lemma expanded_tLambda_inv Σ Γ na t b :
+  expanded Σ Γ (tLambda na t b) ->
+  expanded Σ (0 :: Γ) b.
+Proof.
+  intros exp; depind exp; solve_discr => //; eauto.
+Qed.
+
+Lemma expanded_tLetIn_inv Σ Γ na t t' b :
+  expanded Σ Γ (tLetIn na t t' b) ->
+  expanded Σ Γ t /\ expanded Σ (0 :: Γ) b.
+Proof.
+  intros exp; depind exp; solve_discr => //; eauto.
+Qed.
+
+Lemma expanded_tEvar_inv Σ Γ ev l:
+  expanded Σ Γ (tEvar ev l) ->
+  Forall (expanded Σ Γ) l.
+Proof.
+  intros exp; depind exp; solve_discr => //; eauto.
+Qed.
+
+Lemma expanded_tCase_inv Σ Γ ci p c brs :
+  expanded Σ Γ (tCase ci p c brs) ->
+  Forall (expanded Σ Γ) (pparams p) /\
+  Forall
+    (fun br : branch term =>
+     ∥ All_fold
+         (fun (Δ : list context_decl) (d : context_decl)
+          =>
+          ForOption
+            (fun b : term =>
+             expanded Σ
+               (repeat 0 #|Δ| ++
+                repeat 0 #|pparams p|) b)
+            (decl_body d)) (bcontext br) ∥ /\
+     expanded Σ (repeat 0 #|bcontext br| ++ Γ) (bbody br))
+    brs /\
+  expanded Σ Γ c.
+Proof.
+  intros exp; depind exp; solve_discr => //; eauto.
+Qed.
+
+Lemma expanded_tProj_inv Σ Γ p c :
+  expanded Σ Γ (tProj p c) ->
+  expanded Σ Γ c.
+Proof.
+  intros exp; depind exp; solve_discr => //; eauto.
+Qed.
+
+Lemma expanded_tCoFix_inv Σ Γ mfix idx :
+ expanded Σ Γ (tCoFix mfix idx) ->
+ Forall (fun d : def term => expanded Σ (repeat 0 #|mfix| ++ Γ) (dbody d)) mfix.
+Proof.
+  intros exp; depind exp; solve_discr => //; eauto.
+Qed.
+
+Import PCUICOnOne.
+
+Module Red1Apps.
+
+  Set Warnings "-notation-overridden".
+
+  Inductive red1 (Σ : global_env) (Γ : context) : term -> term -> Type :=
+  (** Reductions *)
+  (** Beta *)
+  | red_beta na t b a ts :
+    Σ ;;; Γ |- mkApps (tLambda na t b) (a :: ts) ⇝ mkApps (b {0 := a}) ts
+
+  (** Let *)
+  | red_zeta na b t b' :
+    Σ ;;; Γ |- tLetIn na b t b' ⇝ b' {0 := b}
+
+  | red_rel i body :
+      option_map decl_body (nth_error Γ i) = Some (Some body) ->
+      Σ ;;; Γ |- tRel i ⇝ lift0 (S i) body
+
+  (** Case *)
+  | red_iota ci c u args p brs br :
+      nth_error brs c = Some br ->
+      #|args| = (ci.(ci_npar) + context_assumptions br.(bcontext))%nat ->
+      Σ ;;; Γ |- tCase ci p (mkApps (tConstruct ci.(ci_ind) c u) args) brs
+          ⇝ iota_red ci.(ci_npar) p args br
+
+  (** Fix unfolding, with guard *)
+  | red_fix mfix idx args narg fn :
+      unfold_fix mfix idx = Some (narg, fn) ->
+      is_constructor narg args = true ->
+      Σ ;;; Γ |- mkApps (tFix mfix idx) args ⇝ mkApps fn args
+
+  (** CoFix-case unfolding *)
+  | red_cofix_case ip p mfix idx args narg fn brs :
+      unfold_cofix mfix idx = Some (narg, fn) ->
+      Σ ;;; Γ |- tCase ip p (mkApps (tCoFix mfix idx) args) brs ⇝
+          tCase ip p (mkApps fn args) brs
+
+  (** CoFix-proj unfolding *)
+  | red_cofix_proj p mfix idx args narg fn :
+      unfold_cofix mfix idx = Some (narg, fn) ->
+      Σ ;;; Γ |- tProj p (mkApps (tCoFix mfix idx) args) ⇝ tProj p (mkApps fn args)
+
+  (** Constant unfolding *)
+  | red_delta c decl body (isdecl : declared_constant Σ c decl) u :
+      decl.(cst_body) = Some body ->
+      Σ ;;; Γ |- tConst c u ⇝ subst_instance u body
+
+  (** Proj *)
+  | red_proj p args u arg:
+      nth_error args (p.(proj_npars) + p.(proj_arg)) = Some arg ->
+      Σ ;;; Γ |- tProj p (mkApps (tConstruct p.(proj_ind) 0 u) args) ⇝ arg
+
+
+  | abs_red_l na M M' N : Σ ;;; Γ |- M ⇝ M' -> Σ ;;; Γ |- tLambda na M N ⇝ tLambda na M' N
+  | abs_red_r na M M' N : Σ ;;; Γ ,, vass na N |- M ⇝ M' -> Σ ;;; Γ |- tLambda na N M ⇝ tLambda na N M'
+
+  | letin_red_def na b t b' r : Σ ;;; Γ |- b ⇝ r -> Σ ;;; Γ |- tLetIn na b t b' ⇝ tLetIn na r t b'
+  | letin_red_ty na b t b' r : Σ ;;; Γ |- t ⇝ r -> Σ ;;; Γ |- tLetIn na b t b' ⇝ tLetIn na b r b'
+  | letin_red_body na b t b' r : Σ ;;; Γ ,, vdef na b t |- b' ⇝ r -> Σ ;;; Γ |- tLetIn na b t b' ⇝ tLetIn na b t r
+
+  | case_red_param ci p params' c brs :
+      OnOne2 (fun t u => Σ ;;; Γ |- t ⇝ u) p.(pparams) params' ->
+      Σ ;;; Γ |- tCase ci p c brs ⇝ tCase ci (set_pparams p params') c brs
+
+  | case_red_return ci p preturn' c brs :
+    Σ ;;; Γ ,,, inst_case_predicate_context p |- p.(preturn) ⇝ preturn' ->
+    Σ ;;; Γ |- tCase ci p c brs ⇝ tCase ci (set_preturn p preturn') c brs
+
+  | case_red_discr ci p c c' brs :
+    Σ ;;; Γ |- c ⇝ c' -> Σ ;;; Γ |- tCase ci p c brs ⇝ tCase ci p c' brs
+
+  | case_red_brs ci p c brs brs' :
+      OnOne2 (fun br br' =>
+        on_Trel_eq (fun t u => Σ ;;; Γ ,,, inst_case_branch_context p br |- t ⇝ u) bbody bcontext br br')
+        brs brs' ->
+      Σ ;;; Γ |- tCase ci p c brs ⇝ tCase ci p c brs'
+
+  | proj_red p c c' : Σ ;;; Γ |- c ⇝ c' -> Σ ;;; Γ |- tProj p c ⇝ tProj p c'
+
+  | app_red_l M1 N1 M2 : Σ ;;; Γ |- M1 ⇝ N1 -> ~~ isApp M1 -> ~~ isFix M1 -> M2 <> nil ->
+    Σ ;;; Γ |- mkApps M1 M2 ⇝ mkApps N1 M2
+
+  | app_red_r M2 N2 M1 : ~~ isApp M1 -> OnOne2 (fun M2 N2 => Σ ;;; Γ |- M2 ⇝ N2) M2 N2 -> Σ ;;; Γ |- mkApps M1 M2 ⇝ mkApps M1 N2
+
+  | app_fix_red_ty mfix0 mfix1 idx M2 :
+    OnOne2 (on_Trel_eq (fun t u => Σ ;;; Γ |- t ⇝ u) dtype (fun x => (dname x, dbody x, rarg x))) mfix0 mfix1 ->
+    Σ ;;; Γ |- mkApps (tFix mfix0 idx) M2 ⇝ mkApps (tFix mfix1 idx) M2
+
+  | app_fix_red_body mfix0 mfix1 idx M2 :
+    OnOne2 (on_Trel_eq (fun t u => Σ ;;; Γ ,,, fix_context mfix0 |- t ⇝ u) dbody (fun x => (dname x, dtype x, rarg x))) mfix0 mfix1 ->
+    Σ ;;; Γ |- mkApps (tFix mfix0 idx) M2 ⇝ mkApps (tFix mfix1 idx) M2
+
+  | prod_red_l na M1 M2 N1 : Σ ;;; Γ |- M1 ⇝ N1 -> Σ ;;; Γ |- tProd na M1 M2 ⇝ tProd na N1 M2
+  | prod_red_r na M2 N2 M1 : Σ ;;; Γ ,, vass na M1 |- M2 ⇝ N2 ->
+                            Σ ;;; Γ |- tProd na M1 M2 ⇝ tProd na M1 N2
+
+  | evar_red ev l l' : OnOne2 (fun t u => Σ ;;; Γ |- t ⇝ u) l l' -> Σ ;;; Γ |- tEvar ev l ⇝ tEvar ev l'
+
+  | fix_red_ty mfix0 mfix1 idx :
+      OnOne2 (on_Trel_eq (fun t u => Σ ;;; Γ |- t ⇝ u) dtype (fun x => (dname x, dbody x, rarg x))) mfix0 mfix1 ->
+      Σ ;;; Γ |- tFix mfix0 idx ⇝ tFix mfix1 idx
+
+  | fix_red_body mfix0 mfix1 idx :
+      OnOne2 (on_Trel_eq (fun t u => Σ ;;; Γ ,,, fix_context mfix0 |- t ⇝ u) dbody (fun x => (dname x, dtype x, rarg x)))
+            mfix0 mfix1 ->
+      Σ ;;; Γ |- tFix mfix0 idx ⇝ tFix mfix1 idx
+
+  | cofix_red_ty mfix0 mfix1 idx :
+      OnOne2 (on_Trel_eq (fun t u => Σ ;;; Γ |- t ⇝ u) dtype (fun x => (dname x, dbody x, rarg x))) mfix0 mfix1 ->
+      Σ ;;; Γ |- tCoFix mfix0 idx ⇝ tCoFix mfix1 idx
+
+  | cofix_red_body mfix0 mfix1 idx :
+      OnOne2 (on_Trel_eq (fun t u => Σ ;;; Γ ,,, fix_context mfix0 |- t ⇝ u) dbody (fun x => (dname x, dtype x, rarg x))) mfix0 mfix1 ->
+      Σ ;;; Γ |- tCoFix mfix0 idx ⇝ tCoFix mfix1 idx
+  where " Σ ;;; Γ |- t ⇝ u " := (red1 Σ Γ t u).
+
+  Lemma red1_ind_all :
+    forall (Σ : global_env) (P : context -> term -> term -> Type),
+
+       (forall (Γ : context) (na : aname) (t b a : term) ts,
+        P Γ (mkApps (tLambda na t b) (a :: ts)) (mkApps (b {0 := a}) ts)) ->
+
+       (forall (Γ : context) (na : aname) (b t b' : term), P Γ (tLetIn na b t b') (b' {0 := b})) ->
+
+       (forall (Γ : context) (i : nat) (body : term),
+        option_map decl_body (nth_error Γ i) = Some (Some body) -> P Γ (tRel i) ((lift0 (S i)) body)) ->
+
+       (forall (Γ : context) (ci : case_info) (c : nat) (u : Instance.t) (args : list term)
+          (p : predicate term) (brs : list (branch term)) br,
+          nth_error brs c = Some br ->
+          #|args| = (ci.(ci_npar) + context_assumptions br.(bcontext))%nat ->
+          P Γ (tCase ci p (mkApps (tConstruct ci.(ci_ind) c u) args) brs)
+              (iota_red ci.(ci_npar) p args br)) ->
+
+       (forall (Γ : context) (mfix : mfixpoint term) (idx : nat) (args : list term) (narg : nat) (fn : term),
+        unfold_fix mfix idx = Some (narg, fn) ->
+        is_constructor narg args = true -> P Γ (mkApps (tFix mfix idx) args) (mkApps fn args)) ->
+
+       (forall (Γ : context) ci (p : predicate term) (mfix : mfixpoint term) (idx : nat)
+          (args : list term) (narg : nat) (fn : term) (brs : list (branch term)),
+        unfold_cofix mfix idx = Some (narg, fn) ->
+        P Γ (tCase ci p (mkApps (tCoFix mfix idx) args) brs) (tCase ci p (mkApps fn args) brs)) ->
+
+       (forall (Γ : context) (p : projection) (mfix : mfixpoint term) (idx : nat) (args : list term)
+          (narg : nat) (fn : term),
+        unfold_cofix mfix idx = Some (narg, fn) -> P Γ (tProj p (mkApps (tCoFix mfix idx) args)) (tProj p (mkApps fn args))) ->
+
+       (forall (Γ : context) c (decl : constant_body) (body : term),
+        declared_constant Σ c decl ->
+        forall u : Instance.t, cst_body decl = Some body -> P Γ (tConst c u) (subst_instance u body)) ->
+
+       (forall (Γ : context) p (args : list term) (u : Instance.t)
+         (arg : term),
+           nth_error args (p.(proj_npars) + p.(proj_arg)) = Some arg ->
+           P Γ (tProj p (mkApps (tConstruct p.(proj_ind) 0 u) args)) arg) ->
+
+       (forall (Γ : context) (na : aname) (M M' N : term),
+        red1 Σ Γ M M' -> P Γ M M' -> P Γ (tLambda na M N) (tLambda na M' N)) ->
+
+       (forall (Γ : context) (na : aname) (M M' N : term),
+        red1 Σ (Γ,, vass na N) M M' -> P (Γ,, vass na N) M M' -> P Γ (tLambda na N M) (tLambda na N M')) ->
+
+       (forall (Γ : context) (na : aname) (b t b' r : term),
+        red1 Σ Γ b r -> P Γ b r -> P Γ (tLetIn na b t b') (tLetIn na r t b')) ->
+
+       (forall (Γ : context) (na : aname) (b t b' r : term),
+        red1 Σ Γ t r -> P Γ t r -> P Γ (tLetIn na b t b') (tLetIn na b r b')) ->
+
+       (forall (Γ : context) (na : aname) (b t b' r : term),
+        red1 Σ (Γ,, vdef na b t) b' r -> P (Γ,, vdef na b t) b' r -> P Γ (tLetIn na b t b') (tLetIn na b t r)) ->
+
+       (forall (Γ : context) (ci : case_info) p params' c brs,
+          OnOne2 (Trel_conj (red1 Σ Γ) (P Γ)) p.(pparams) params' ->
+           P Γ (tCase ci p c brs)
+               (tCase ci (set_pparams p params') c brs)) ->
+
+       (forall (Γ : context) (ci : case_info) p preturn' c brs,
+          red1 Σ (Γ ,,, inst_case_predicate_context p) p.(preturn) preturn' ->
+          P (Γ ,,, inst_case_predicate_context p) p.(preturn) preturn' ->
+          P Γ (tCase ci p c brs)
+              (tCase ci (set_preturn p preturn') c brs)) ->
+
+       (forall (Γ : context) (ind : case_info) (p : predicate term) (c c' : term) (brs : list (branch term)),
+        red1 Σ Γ c c' -> P Γ c c' -> P Γ (tCase ind p c brs) (tCase ind p c' brs)) ->
+
+       (forall (Γ : context) ci p c brs brs',
+          OnOne2 (fun br br' =>
+          (on_Trel_eq (Trel_conj (red1 Σ (Γ ,,, inst_case_branch_context p br))
+            (P (Γ ,,, inst_case_branch_context p br)))
+            bbody bcontext br br')) brs brs' ->
+          P Γ (tCase ci p c brs) (tCase ci p c brs')) ->
+
+       (forall (Γ : context) (p : projection) (c c' : term), red1 Σ Γ c c' -> P Γ c c' ->
+                                                             P Γ (tProj p c) (tProj p c')) ->
+
+       (forall (Γ : context) M1 N1 M2, red1 Σ Γ M1 N1 -> P Γ M1 N1 -> ~~ isApp M1 -> ~~ isFix M1 -> M2 <> [] ->
+                                                         P Γ (mkApps M1 M2) (mkApps N1 M2)) ->
+
+       (forall (Γ : context) M1 N2 M2, ~~ isApp M1 ->
+        OnOne2 (Trel_conj (red1 Σ Γ) (P Γ)) M2 N2 ->
+        P Γ (mkApps M1 M2) (mkApps M1 N2)) ->
+
+      (forall (Γ : context) mfix0 mfix1 idx M2,
+        OnOne2 (on_Trel_eq (Trel_conj (fun t u => Σ ;;; Γ |- t ⇝ u) (P Γ)) dtype (fun x => (dname x, dbody x, rarg x))) mfix0 mfix1 ->
+        P Γ (mkApps (tFix mfix0 idx) M2) (mkApps (tFix mfix1 idx) M2)) ->
+
+      (forall (Γ : context) mfix0 mfix1 idx M2,
+        OnOne2 (on_Trel_eq (Trel_conj (fun t u => Σ ;;; Γ ,,, fix_context mfix0 |- t ⇝ u) (P (Γ ,,, fix_context mfix0))) dbody (fun x => (dname x, dtype x, rarg x))) mfix0 mfix1 ->
+        P Γ (mkApps (tFix mfix0 idx) M2) (mkApps (tFix mfix1 idx) M2)) ->
+
+       (forall (Γ : context) (na : aname) (M1 M2 N1 : term),
+        red1 Σ Γ M1 N1 -> P Γ M1 N1 -> P Γ (tProd na M1 M2) (tProd na N1 M2)) ->
+
+       (forall (Γ : context) (na : aname) (M2 N2 M1 : term),
+        red1 Σ (Γ,, vass na M1) M2 N2 -> P (Γ,, vass na M1) M2 N2 -> P Γ (tProd na M1 M2) (tProd na M1 N2)) ->
+
+       (forall (Γ : context) (ev : nat) (l l' : list term),
+           OnOne2 (Trel_conj (red1 Σ Γ) (P Γ)) l l' -> P Γ (tEvar ev l) (tEvar ev l')) ->
+
+       (forall (Γ : context) (mfix0 mfix1 : list (def term)) (idx : nat),
+        OnOne2 (on_Trel_eq (Trel_conj (red1 Σ Γ) (P Γ)) dtype (fun x => (dname x, dbody x, rarg x))) mfix0 mfix1 ->
+        P Γ (tFix mfix0 idx) (tFix mfix1 idx)) ->
+
+       (forall (Γ : context) (mfix0 mfix1 : list (def term)) (idx : nat),
+        OnOne2 (on_Trel_eq (Trel_conj (red1 Σ (Γ ,,, fix_context mfix0))
+                                      (P (Γ ,,, fix_context mfix0))) dbody
+                           (fun x => (dname x, dtype x, rarg x))) mfix0 mfix1 ->
+        P Γ (tFix mfix0 idx) (tFix mfix1 idx)) ->
+
+       (forall (Γ : context) (mfix0 mfix1 : list (def term)) (idx : nat),
+        OnOne2 (on_Trel_eq (Trel_conj (red1 Σ Γ) (P Γ)) dtype (fun x => (dname x, dbody x, rarg x))) mfix0 mfix1 ->
+        P Γ (tCoFix mfix0 idx) (tCoFix mfix1 idx)) ->
+
+       (forall (Γ : context) (mfix0 mfix1 : list (def term)) (idx : nat),
+        OnOne2 (on_Trel_eq (Trel_conj (red1 Σ (Γ ,,, fix_context mfix0))
+                                      (P (Γ ,,, fix_context mfix0))) dbody
+                           (fun x => (dname x, dtype x, rarg x))) mfix0 mfix1 ->
+        P Γ (tCoFix mfix0 idx) (tCoFix mfix1 idx)) ->
+
+       forall (Γ : context) (t t0 : term), red1 Σ Γ t t0 -> P Γ t t0.
+  Proof.
+    intros. rename X29 into Xlast. revert Γ t t0 Xlast.
+    fix aux 4. intros Γ t T.
+    move aux at top.
+    destruct 1; match goal with
+                | |- P _ (tFix _ _) (tFix _ _) => idtac
+                | |- P _ (tCoFix _ _) (tCoFix _ _) => idtac
+                | |- P _ (mkApps (tFix _ _) _) _ => idtac
+                | |- P _ (tCase _ _ (mkApps (tCoFix _ _) _) _) _ => idtac
+                | |- P _ (tProj _ (mkApps (tCoFix _ _) _)) _ => idtac
+                | H : _ |- _ => eapply H; eauto
+                end.
+    - eapply X3; eauto.
+    - eapply X4; eauto.
+    - eapply X5; eauto.
+
+    - revert params' o.
+      generalize (pparams p).
+      fix auxl 3.
+      intros params params' [].
+      + constructor. split; auto.
+      + constructor. auto.
+
+    - revert brs' o.
+      revert brs.
+      fix auxl 3.
+      intros l l' Hl. destruct Hl.
+      + simpl in *. constructor; intros; intuition auto.
+      + constructor. eapply auxl. apply Hl.
+
+    - revert M2 N2 o.
+      fix auxl 3.
+      intros l l' Hl. destruct Hl.
+      + constructor. split; auto.
+      + constructor. auto.
+
+    - eapply X20.
+      revert mfix0 mfix1 o.
+      fix auxl 3.
+      intros l l' Hl. destruct Hl.
+      + constructor; split; auto; intuition.
+      + constructor; try split; auto; intuition.
+
+    - eapply X21. revert o.
+      generalize (fix_context mfix0).
+      intros c o. revert mfix0 mfix1 o.
+      fix auxl 3.
+      intros l l' Hl. destruct Hl.
+      + constructor. split; auto; intuition.
+      + constructor; try split; auto; intuition.
+
+    - revert l l' o.
+      fix auxl 3.
+      intros l l' Hl. destruct Hl.
+      + constructor. split; auto.
+      + constructor. auto.
+
+    - eapply X25.
+      revert mfix0 mfix1 o; fix auxl 3.
+      intros l l' Hl; destruct Hl;
+      constructor; try split; auto; intuition.
+
+    - eapply X26.
+      revert o. generalize (fix_context mfix0). intros c Xnew.
+      revert mfix0 mfix1 Xnew; fix auxl 3; intros l l' Hl;
+      destruct Hl; constructor; try split; auto; intuition.
+
+    - eapply X27.
+      revert mfix0 mfix1 o.
+      fix auxl 3; intros l l' Hl; destruct Hl;
+        constructor; try split; auto; intuition.
+
+    - eapply X28.
+      revert o. generalize (fix_context mfix0). intros c new.
+      revert mfix0 mfix1 new; fix auxl 3; intros l l' Hl; destruct Hl;
+        constructor; try split; auto; intuition.
+  Defined.
+
+  Lemma red_tApp Σ Γ t v u :
+    red1 Σ Γ t v ->
+    red1 Σ Γ (tApp t u) (tApp v u).
+  Proof.
+    induction 1.
+    all:try solve [eapply (app_red_l _ _ _ _ [u]) => //; econstructor; eauto].
+    - rewrite -![tApp _ u](mkApps_app _ _ [u]).
+      eapply red_beta.
+    - rewrite -![tApp _ u](mkApps_app _ _ [u]). econstructor; eauto.
+      now apply is_constructor_app_ge.
+    - rewrite -![tApp _ u](mkApps_app _ _ [u]). econstructor; eauto.
+    - rewrite -![tApp _ u](mkApps_app _ _ [u]). econstructor; eauto.
+      now eapply OnOne2_app_r.
+    - rewrite -![tApp _ u](mkApps_app _ _ [u]). now eapply app_fix_red_ty.
+    - rewrite -![tApp _ u](mkApps_app _ _ [u]). now eapply app_fix_red_body.
+    - now eapply (app_fix_red_ty _ _ _ _ _ [_]).
+    - now eapply (app_fix_red_body _ _ _ _ _ [_]).
+  Qed.
+
+  Lemma isLambda_red1 Σ Γ b b' : isLambda b -> red1 Σ Γ b b' -> isLambda b'.
+  Proof.
+    destruct b; simpl; try discriminate.
+    intros _ red.
+    depelim red; solve_discr; eauto. depelim o.
+  Qed.
+
+End Red1Apps.
+
+Lemma red1_red1apps Σ Γ t v :
+  red1 Σ Γ t v -> Red1Apps.red1 Σ Γ t v.
+Proof.
+  intros red; induction red using red1_ind_all in |- *.
+  all:try solve [econstructor; eauto; solve_all; eauto].
+  - eapply (Red1Apps.red_beta _ _ _ _ _ _ []).
+  - now eapply Red1Apps.red_tApp.
+  - remember (decompose_app (tApp M1 M2)).
+    destruct p as [hd args].
+    edestruct (decompose_app_rec_inv' M1 [M2]). rewrite /decompose_app in Heqp.
+    cbn in Heqp. rewrite -Heqp. reflexivity.
+    destruct a as [napp [hm2 hm1]].
+    symmetry in Heqp; eapply decompose_app_inv in Heqp. rewrite Heqp.
+    assert (tApp M1 N2 = mkApps hd (firstn x args ++ [N2])) as ->.
+    { now rewrite mkApps_app -hm1. }
+    rewrite -{1}(firstn_skipn x args) -hm2. eapply Red1Apps.app_red_r => //.
+    eapply OnOne2_app. now constructor.
+Qed.
+
+Lemma head_nApp f :
+  ~~ isApp f -> head f = f.
+Proof.
+  induction f => //.
+Qed.
+
+Lemma expanded_mkApps_inv Σ Γ f v :
+  ~~ isApp f ->
+  ~~ (isConstruct f || isFix f || isRel f) ->
+  expanded Σ Γ (mkApps f v) ->
+  expanded Σ Γ f /\ Forall (expanded Σ Γ) v.
+Proof.
+  intros happ hc.
+  induction v using rev_ind; cbn.
+  - intros exp; split => //.
+  - rewrite mkApps_app /=.
+    move/expanded_tApp_inv => e.
+    forward e. rewrite head_mkApps.
+    rewrite head_nApp //. now move/negbTE: hc ->.
+    intuition auto. eapply app_Forall; eauto.
+Qed.
+
+Lemma expanded_mkApps_inv' Σ Γ f :
+  expanded Σ Γ f ->
+  let args := arguments f in
+  Forall (expanded Σ Γ) args /\
+    match head f with
+    | tRel n => exists m, nth_error Γ n = Some m /\ m <= #|args|
+    | tConstruct ind c u => exists mind idecl cdecl,
+      declared_constructor Σ (ind, c) mind idecl cdecl /\ #|args| >= ind_npars mind + context_assumptions (cstr_args cdecl)
+    | tFix mfix idx => exists d,
+      Forall
+        (fun d0 : def term =>
+        isLambda (dbody d0) /\
+        (let ctx :=
+            rev_map (fun d1 : def term => (1 + rarg d1)%nat)
+              mfix in
+          expanded Σ (ctx ++ Γ) (dbody d0))) mfix /\
+      args <> [] /\
+      nth_error mfix idx = Some d /\ #|args| > rarg d
+    | _ => expanded Σ Γ (head f)
+    end.
+Proof.
+  induction 1 using expanded_ind; cbn.
+  all: try solve [split; econstructor; eauto].
+  all:rewrite head_mkApps /=.
+  - rewrite arguments_mkApps_nApp //. split => //. now exists m.
+  - destruct IHexpanded. rewrite arguments_mkApps. split.
+    eapply app_Forall => //.
+    rewrite app_length.
+    destruct (head f6) => //; firstorder (eauto; try lia).
+    exists x. split => //. firstorder (eauto; try lia).
+    intros heq; apply H5. now eapply app_eq_nil in heq.
+  - rewrite arguments_mkApps_nApp //. split => //. now exists d.
+  - rewrite arguments_mkApps_nApp //. split => //.
+    firstorder.
+Qed.
+
+Lemma All_fold_map_context (P : context -> context_decl -> Type) (f : term -> term) ctx :
+  All_fold P (map_context f ctx) <~> All_fold (fun Γ d => P (map_context f Γ) (map_decl f d)) ctx.
+Proof.
+  induction ctx.
+  - split; constructor.
+  - cbn. split; intros H; depelim H; constructor; auto; now apply IHctx.
+Qed.
+
+Lemma expanded_fix_subst Σ a k b Γ Γs Δ :
+  #|Γ| = k ->
+  Forall2 (fun n arg => forall args Γ' k',
+    Forall (expanded Σ (Γ' ++ Δ)) args ->
+    n <= #|args| ->
+    #|Γ'| = k' ->
+    expanded Σ (Γ' ++ Δ) (mkApps (lift0 k' arg) args)) Γs a ->
+  expanded Σ (Γ ++ Γs ++ Δ) b ->
+  expanded Σ (Γ ++ Δ) (subst a k b).
+Proof.
+  intros Hk Hs.
+  remember (Γ ++ _ ++ Δ)%list as Γ_.
+  intros exp; revert Γ k Hk HeqΓ_.
+  induction exp using expanded_ind; intros Γ' k Hk ->.
+  all:try solve[ cbn; econstructor => // ].
+  2,7:solve[ cbn; econstructor => //; solve_all ].
+  - rewrite subst_mkApps /=.
+    destruct (Nat.leb_spec k n).
+    destruct (nth_error a _) eqn:hnth.
+    * pose proof (Forall2_length Hs).
+      pose proof (Forall2_nth_error_Some_r _ _ _ _ _ _ _ hnth Hs) as [t' [hnth' hargs]].
+      eapply hargs => //.
+      eapply Forall_map.
+      2:{ len. rewrite nth_error_app_ge in H. lia. subst k.
+        rewrite nth_error_app_lt in H.
+        eapply nth_error_Some_length in hnth'. lia. rewrite hnth' in H. noconf H. exact H0. }
+      solve_all.
+    * rewrite nth_error_app_ge in H. lia.
+      eapply nth_error_None in hnth.
+      pose proof (Forall2_length Hs).
+      rewrite nth_error_app_ge in H. lia.
+      eapply expanded_tRel. rewrite nth_error_app_ge. lia. erewrite <- H.
+      lia_f_equal. len. solve_all.
+    * rewrite nth_error_app_lt in H. lia.
+      eapply expanded_tRel. rewrite nth_error_app_lt. lia. tea. now len.
+      solve_all.
+  - cbn. econstructor.
+    eapply (IHexp (0 :: Γ') (S k)); cbn; auto; try lia.
+  - cbn. econstructor. apply IHexp1; auto.
+    eapply (IHexp2 (0 :: Γ') (S k)); cbn; auto; lia.
+  - rewrite subst_mkApps.
+    destruct (isConstruct (subst a k f6) || isFix (subst a k f6) || isRel (subst a k f6)) eqn:eqc.
+    specialize (IHexp  _ _ Hk eq_refl).
+    eapply expanded_mkApps_expanded => //. solve_all.
+    eapply expanded_mkApps => //. rewrite eqc //. now eapply IHexp. solve_all.
+  - cbn. econstructor. eauto. cbn. solve_all. solve_all.
+    specialize (H1 (repeat 0 #|bcontext x| ++ Γ') (#|bcontext x| + k)%nat).
+    forward H1 by len.
+    forward H1. now rewrite app_assoc.
+    rewrite /id. rewrite app_assoc. apply H1.
+  - rewrite subst_mkApps. cbn.
+    eapply expanded_tFix.
+    + solve_all. now eapply isLambda_subst.
+      specialize (a0
+      (rev_map (fun d0 : def term => S (rarg d0))
+      (map (map_def (subst a k) (subst a (#|mfix| + k))) mfix) ++ Γ') (#|mfix| + k)%nat).
+      forward a0 by len.
+      forward a0. { rewrite app_assoc. f_equal. f_equal.
+        rewrite !rev_map_spec. f_equal. now rewrite map_map_compose /=. }
+      rewrite app_assoc. eapply a0.
+    + solve_all.
+    + now destruct args.
+    + rewrite nth_error_map /= H4 //.
+    + len.
+  - cbn. constructor.
+    solve_all.
+    specialize (a0 (repeat 0 #|mfix| ++ Γ') (#|mfix| + k)%nat).
+    forward a0 by len.
+    forward a0. { rewrite app_assoc //. }
+    rewrite app_assoc. eapply a0.
+  - rewrite subst_mkApps. cbn.
+    eapply expanded_tConstruct_app; tea. now len.
+    solve_all.
+Qed.
+
+Lemma expanded_unfold_fix Σ Γ' mfix idx narg fn :
+  unfold_fix mfix idx = Some (narg, fn) ->
+  All (fun d0 : def term => isLambda (dbody d0) /\ expanded Σ (rev_map (fun d1 : def term => S (rarg d1)) mfix ++ Γ') (dbody d0)) mfix ->
+  expanded Σ Γ' fn.
+Proof.
+  unfold unfold_fix.
+  destruct nth_error eqn:e => //.
+  intros [= <- <-] hf.
+  pose proof (nth_error_all e hf) as [hl hf'].
+  eapply (expanded_fix_subst _ _ _ _ []) => //; tea.
+  rewrite rev_map_spec.
+  eapply Forall2_from_nth_error. len.
+  intros n rarg f. len. intros hn hrarg hnthf args Γ'' k' hargs hrarg' <-.
+  eapply PCUICParallelReductionConfluence.nth_error_fix_subst in hnthf. subst f.
+  move: hrarg.
+  rewrite nth_error_rev; len. rewrite List.rev_involutive nth_error_map.
+  intros hrarg.
+  destruct (nth_error mfix (_ - _)) eqn:e'. cbn in hrarg. noconf hrarg.
+  eapply expanded_tFix => //. solve_all.
+  eapply expanded_lift; len. rewrite !rev_map_spec in H1 *.
+  rewrite map_map => //. destruct args => //. cbn in hrarg'. lia.
+  rewrite nth_error_map /= e' /= //. cbn. lia.
+  eapply nth_error_None in e'. lia.
+Qed.
+
+Lemma expanded_unfold_cofix Σ Γ' mfix idx narg fn :
+  unfold_cofix mfix idx = Some (narg, fn) ->
+  All (fun d0 : def term => expanded Σ (repeat 0 #|mfix| ++ Γ') (dbody d0)) mfix ->
+  expanded Σ Γ' fn.
+Proof.
+  unfold unfold_cofix.
+  destruct nth_error eqn:e => //.
+  intros [= <- <-] hf.
+  pose proof (nth_error_all e hf) as hf'.
+  eapply (expanded_subst _ _ _ _ []) => //; tea.
+  rewrite /cofix_subst.
+  generalize #|mfix|.
+  induction n; repeat constructor; eauto. solve_all.
+  len.
+Qed.
+
+Lemma expanded_weakening_env {cf : checker_flags} Σ Σ' Γ t :
+  wf Σ' ->
+  extends Σ Σ' ->
+  expanded Σ Γ t -> expanded Σ' Γ t.
+Proof.
+  intros w s.
+  eapply expanded_ind; intros.
+  all:try solve [econstructor; eauto].
+  - econstructor; eauto. solve_all. sq. eapply All_fold_impl; tea. cbn.
+    intros. now rewrite repeat_app in H6.
+  - eapply expanded_tFix; eauto. solve_all.
+  - eapply expanded_tConstruct_app; eauto.
+    eapply PCUICWeakeningEnv.weakening_env_declared_constructor; tea.
+Qed.
+
+Lemma expanded_global_env_constant {cf : checker_flags} Σ c decl :
+  wf Σ ->
+  expanded_global_env Σ ->
+  declared_constant Σ c decl ->
+  ForOption (expanded Σ []) (cst_body decl).
+Proof.
+  intros wf; destruct Σ as [Σ univs] => /=. cbn.
+  unfold expanded_global_env. cbn.
+  induction 1; cbn => //.
+  intros [->|H'].
+  - depelim H0.
+    destruct decl as [? [] ?]; cbn in *.
+    constructor. cbn.
+    eapply expanded_weakening_env; tea.
+    eapply extends_strictly_on_decls_extends.
+    split => //=. eapply incl_cs_refl. 2:eapply Retroknowledge.extends_refl.
+    set (cb := ConstantDecl _). now exists [(c, cb)].
+    constructor.
+  - forward IHexpanded_global_declarations.
+    destruct wf. cbn in *. split => //.
+    cbn. now depelim o0.
+    eapply IHexpanded_global_declarations in H'.
+    destruct decl as [? [] ?]; cbn in * => //. 2:constructor.
+    depelim H'. constructor.
+    eapply expanded_weakening_env; tea.
+    eapply extends_strictly_on_decls_extends.
+    split => //=. eapply incl_cs_refl. 2:eapply Retroknowledge.extends_refl.
+    now exists [decl0].
+Qed.
+
+Lemma All_fold_nth_error P (ctx : context) n b :
+  All_fold P ctx -> nth_error ctx n = Some b ->
+  P (skipn (S n) ctx) b.
+Proof.
+  induction 1 in n, b |- *.
+  - rewrite nth_error_nil //.
+  - destruct n => //=.
+    * intros [= <-]. now rewrite skipn_S skipn_0.
+    * intros hnth. now rewrite skipn_S.
+Qed.
+
+Lemma skipn_repeat {A} k n (a : A) :
+  skipn n (repeat a k) = repeat a (k - n).
+Proof.
+  induction n in k |- *.
+  - rewrite skipn_0. lia_f_equal.
+  - destruct k => //=.
+    rewrite skipn_S IHn. lia_f_equal.
+Qed.
+
+Lemma expanded_red1 {cf : checker_flags} {Σ : global_env_ext} Γ Γ' t v : wf Σ ->
+  expanded_global_env Σ ->
+  (forall n body, option_map decl_body (nth_error Γ n) = Some (Some body) -> expanded Σ (skipn (S n) Γ') body) ->
+  red1 Σ Γ t v ->
+  expanded Σ Γ' t ->
+  expanded Σ Γ' v.
+Proof.
+  move=> wf expΣ wfΓ /red1_red1apps red.
+  induction red using Red1Apps.red1_ind_all in wfΓ, Γ' |- *;  intros exp.
+  - eapply expanded_mkApps_inv in exp as [] => //.
+    eapply expanded_tLambda_inv in H.
+    depelim H0.
+    eapply expanded_mkApps_expanded => //.
+    eapply (expanded_subst _ _ _ _ [] Γ') => //. now constructor. solve_all.
+  - eapply expanded_tLetIn_inv in exp as [].
+    eapply (expanded_subst _ _ _ _ [] Γ') => //. now constructor.
+  - rewrite -(firstn_skipn (S i) Γ').
+    eapply expanded_mkApps_inv' in exp; cbn in exp.
+    destruct exp as [_ [m []]]. eapply nth_error_Some_length in H0.
+    eapply (expanded_lift _ _ _ _ []) => //.
+    rewrite firstn_length_le; try lia.
+    now eapply wfΓ.
+  - eapply expanded_tCase_inv in exp as [? []].
+    unfold iota_red.
+    move/expanded_mkApps_inv': H3 => /=.
+    rewrite arguments_mkApps_nApp // head_mkApps //=.
+    intros [hargs [mind [idecl [cdecl [declc hargs']]]]].
+    eapply nth_error_forall in H2; tea.
+    destruct H2 as [[hbctx] hbod].
+    eapply (expanded_subst _ _ _ _ [] _) => //.
+    + eapply Forall_rev, Forall_skipn => //.
+    + len. replace #|skipn (ci_npar ci) args| with (context_assumptions (inst_case_branch_context p br)).
+      eapply expanded_let_expansion; len. red.
+      sq. rewrite /inst_case_branch_context /inst_case_context /subst_context.
+      eapply PCUICParallelReduction.All_fold_fold_context_k.
+      eapply All_fold_map_context, All_fold_impl; tea; cbn.
+      intros ? ? fo. len. destruct x as [? [] ?] => //; constructor.
+      cbn in fo. depelim fo. eapply (expanded_subst _ _ _ _ (repeat 0 #|Γ0|) _); len.
+      eapply Forall_rev; eauto.
+      eapply expanded_subst_instance. rewrite app_assoc. now eapply expanded_weakening.
+      rewrite skipn_length. len.
+  - move/expanded_mkApps_inv': exp. cbn.
+    rewrite arguments_mkApps_nApp // head_mkApps //=.
+    move=> [hargs [d [hf [hargs' []]]]] hnth hrarg.
+    eapply expanded_mkApps_expanded => //; solve_all.
+    eapply expanded_unfold_fix in H; tea.
+  - eapply expanded_tCase_inv in exp as [? []].
+    constructor => //.
+    eapply expanded_mkApps_inv' in H2. move: H2; rewrite arguments_mkApps_nApp // head_mkApps //=.
+    intros [hargs' hcof]. cbn in hcof. eapply expanded_tCoFix_inv in hcof.
+    eapply expanded_unfold_cofix in H; tea. eapply expanded_mkApps_expanded; tea => //; solve_all. solve_all.
+  - eapply expanded_tProj_inv in exp. econstructor.
+    eapply expanded_mkApps_inv' in exp. move: exp; rewrite arguments_mkApps_nApp // head_mkApps //=.
+    intros [hargs' hcof]. cbn in hcof. eapply expanded_tCoFix_inv in hcof.
+    eapply expanded_mkApps_expanded => //; solve_all.
+    eapply expanded_unfold_cofix in H; tea.
+  - eapply expanded_subst_instance.
+    eapply expanded_global_env_constant in expΣ; tea.
+    eapply (expanded_weakening _ []). rewrite H0 in expΣ. now depelim expΣ.
+  - eapply expanded_tProj_inv in exp.
+    move/expanded_mkApps_inv': exp. rewrite arguments_mkApps_nApp // head_mkApps //=.
+    intros [].
+    eapply nth_error_forall in H0; tea.
+  - constructor. now eapply expanded_tLambda_inv in exp.
+  - constructor. eapply expanded_tLambda_inv in exp.
+    eapply IHred => //.
+    { intros [] body; cbn => //. rewrite skipn_S. eapply wfΓ. }
+  - eapply expanded_tLetIn_inv in exp; now constructor.
+  - eapply expanded_tLetIn_inv in exp. now constructor.
+  - eapply expanded_tLetIn_inv in exp. constructor; intuition eauto.
+    eapply IHred => //.
+    { intros [] ? => //=. intros [=]. subst b. now rewrite skipn_S skipn_0.
+      rewrite skipn_S. eapply wfΓ. }
+  - eapply expanded_tCase_inv in exp as [? []].
+    constructor; eauto. cbn.
+    solve_all. eapply OnOne2_impl_All_r; tea. intuition eauto. now apply X0.
+    now rewrite /PCUICOnOne.set_pparams /= -(OnOne2_length X).
+  - eapply expanded_tCase_inv in exp as [? []].
+    constructor; eauto.
+  - eapply expanded_tCase_inv in exp as [? []].
+    econstructor; eauto.
+  - eapply expanded_tCase_inv in exp as [? []].
+    econstructor; eauto. solve_all.
+    eapply OnOne2_impl_All_r; tea.
+    intros x y [? ?]. intros [[] ?]. rewrite -e0.
+    solve_all. eapply e => //.
+    intros n b.
+    clear -H H2 wfΓ.
+    destruct nth_error eqn:e' => //.
+    cbn. intros [=]. destruct c as [? [] ?]. cbn in *. noconf H1.
+    eapply nth_error_app_inv in e' as [[]|[]].
+    { rewrite inst_case_branch_context_length in H0. destruct H2.
+      rewrite /inst_case_branch_context /inst_case_context in H1.
+      destruct (nth_error (bcontext x) n) eqn:e.
+      2:{ eapply nth_error_None in e. rewrite skipn_app skipn_all2. len. cbn. len. }
+      rewrite /subst_context in H1.
+      erewrite nth_error_fold_context_k in H1. 4:{ rewrite nth_error_map e //. } 3:len. 2:exact [].
+      len in H1. noconf H1. destruct c as [? [] ?]; noconf H1.
+      rewrite skipn_app. len. eapply All_fold_nth_error in X; tea. cbn in X. depelim X.
+      rewrite skipn_length in H1.
+      eapply expanded_subst. rewrite skipn_length. len.
+      replace (S n - #|bcontext x|) with 0. 2:{ lia. } rewrite skipn_0. eapply Forall_rev. solve_all.
+      len. rewrite app_assoc. eapply expanded_weakening. eapply expanded_subst_instance.
+      now rewrite skipn_repeat. }
+    { rewrite inst_case_branch_context_length in H0, H1.
+      rewrite skipn_app skipn_all2 /=; len.
+      replace (S n - #|bcontext x|) with (S (n - #|bcontext x|)). 2:lia.
+      eapply wfΓ. rewrite H1 //. }
+    noconf H1.
+  - eapply expanded_tProj_inv in exp. now econstructor.
+  - eapply expanded_mkApps_inv' in exp.
+    rewrite head_mkApps head_nApp in exp => //.
+    rewrite arguments_mkApps_nApp // in exp. destruct exp as [].
+    specialize (IHred Γ' wfΓ).
+    destruct M1; try solve [eapply expanded_mkApps_expanded => //; eauto; solve_all].
+    * depelim red; solve_discr. eapply wfΓ in e.
+      eapply expanded_mkApps_expanded => //; solve_all.
+      rewrite -(firstn_skipn (S n) Γ'). eapply (expanded_lift _ _ _ _ []) => //.
+      destruct H3 as [m [hn ha]].
+      rewrite firstn_length_le //. now eapply nth_error_Some_length in hn.
+      depelim o.
+    * depelim red; solve_discr. depelim o.
+
+  - eapply expanded_mkApps_inv' in exp.
+    move: exp.
+    rewrite head_mkApps head_nApp // arguments_mkApps_nApp //.
+    intros [].
+    assert(Forall (expanded Σ Γ') N2).
+    { clear H1. solve_all. eapply OnOne2_impl_All_r; tea. cbn. intuition auto. }
+    destruct M1; try solve [eapply expanded_mkApps => //; eauto].
+    + rewrite (OnOne2_length X) in H1. destruct H1 as [m []]; eapply expanded_tRel; tea.
+    + rewrite (OnOne2_length X) in H1. destruct H1 as [m [? [? []]]]; eapply expanded_tConstruct_app; tea.
+    + rewrite (OnOne2_length X) in H1.
+      destruct H1 as [d [? [? []]]]; eapply expanded_tFix; tea.
+      destruct N2; cbn in *; eauto. lia. intros eq; discriminate.
+
+  - move/expanded_mkApps_inv': exp.
+    rewrite head_mkApps head_nApp // arguments_mkApps_nApp // => [] [] hargs [d [hf [hm2 [hnth harg]]]].
+    eapply OnOne2_nth_error in hnth as [t' [hnth hor]]; tea.
+    eapply expanded_tFix; tea.
+    { clear hor. solve_all. eapply OnOne2_impl_All_r; tea.
+      intros ? ? [] []. noconf e. rewrite -H2. split => //. solve_all.
+      clear -X H1.
+      enough (rev_map (fun d1 : def term => S (rarg d1)) mfix0 = (rev_map (fun d1 : def term => S (rarg d1)) mfix1)) as <- => //.
+      clear -X. rewrite !rev_map_spec. f_equal. induction X. destruct p as []. cbn in *. congruence. cbn. congruence. }
+    { destruct hor; subst => //. destruct p as [? e]; noconf e. now congruence. }
+
+  - move/expanded_mkApps_inv': exp.
+    rewrite head_mkApps head_nApp // arguments_mkApps_nApp // => [] [] hargs [d [hf [hm2 [hnth harg]]]].
+    eapply OnOne2_nth_error in hnth as [t' [hnth hor]]; tea.
+    eapply expanded_tFix; tea.
+    { clear hor. solve_all.
+      assert (rev_map (fun d1 : def term => S (rarg d1)) mfix0 = (rev_map (fun d1 : def term => S (rarg d1)) mfix1)).
+      { clear -X. rewrite !rev_map_spec. f_equal. induction X. destruct p as []. cbn in *. congruence. cbn. congruence. }
+      rewrite -H.
+      eapply OnOne2_impl_All_r; tea.
+      intros ? ? [] []. noconf e. destruct p.
+      eapply Red1Apps.isLambda_red1 in r; tea. split => //.
+      set(Γ'' := rev_map (fun d1 : def term => S (rarg d1)) mfix0).
+      eapply e => //.
+      { intros n b hnth'.
+        destruct (nth_error (fix_context mfix0) n) eqn:e'.
+        rewrite nth_error_app_lt in hnth'. now eapply nth_error_Some_length in e'.
+        rewrite e' in hnth'. noconf hnth'.
+        pose proof (PCUICParallelReductionConfluence.fix_context_assumption_context mfix0).
+        eapply PCUICParallelReductionConfluence.nth_error_assumption_context in H6; tea. congruence.
+        rewrite /Γ''.
+        eapply nth_error_None in e'. len in e'.
+        rewrite nth_error_app_ge in hnth' => //. now len.
+        rewrite skipn_app skipn_all2. len.
+        cbn. len. replace (S n - #|mfix0|) with (S (n - #|mfix0|)). 2:{ lia. }
+        eapply wfΓ. now len in hnth'. } }
+    { destruct hor; subst => //. destruct p as [? e]; noconf e. now congruence. }
+  - eapply expanded_tProd.
+  - constructor.
+  - constructor.
+    eapply expanded_tEvar_inv in exp.
+    solve_all; eapply OnOne2_impl_All_r; tea. intuition eauto.
+    now eapply X0.
+  - depelim exp; solve_discr. now cbn in H.
+  - depelim exp; solve_discr. now cbn in H.
+  - eapply expanded_tCoFix_inv in exp. econstructor.
+    rewrite -(OnOne2_length X). solve_all; eapply OnOne2_impl_All_r; tea; intuition eauto.
+    destruct X0. noconf e. now rewrite -H1.
+  - eapply expanded_tCoFix_inv in exp. econstructor.
+    rewrite -(OnOne2_length X). solve_all; eapply OnOne2_impl_All_r; tea; intuition eauto.
+    destruct X0. destruct p. noconf e. eapply e0 => //.
+    intros n b.
+    destruct nth_error eqn:e' => //.
+    cbn. intros [=]. destruct c as [? [] ?]. cbn in *. noconf H4.
+    eapply nth_error_app_inv in e' as [[]|[]].
+    { pose proof (PCUICParallelReductionConfluence.fix_context_assumption_context mfix0).
+      eapply PCUICParallelReductionConfluence.nth_error_assumption_context in H5; tea. cbn in H5. congruence. }
+    len in H3. len in H4.
+    rewrite skipn_app skipn_all2; len.
+    replace (S n - #|mfix0|) with (S (n - #|mfix0|)) by lia. eapply wfΓ. rewrite H4 /= //.
+    noconf H4.
+Qed.
+
+Lemma expanded_red {cf : checker_flags} {Σ : global_env_ext} Γ Γ' t v : wf Σ ->
+  expanded_global_env Σ ->
+  (forall n body, option_map decl_body (nth_error Γ n) = Some (Some body) -> expanded Σ (skipn (S n) Γ') body) ->
+  red Σ Γ t v ->
+  expanded Σ Γ' t ->
+  expanded Σ Γ' v.
+Proof.
+  intros.
+  induction X0. now eapply expanded_red1. auto.
+  eapply IHX0_2. now eapply IHX0_1.
 Qed.
 
